本题考查了二重积分的计算，属于基础题.解：令

$$
A=\int {}_{(0,0)}^{(1,1)}xydx+(y-x)dy
$$
$$
=\int {}_{(0,0)}^{(1,1)}(xy-y+x-1)dx+(x-1)dy
$$
$$
=(\frac{1}{2}xy^2-xy+x^2-x)dx+(x-1)dy
$$
$$
=(\frac{1}{2}y^2-y+1-1)dx+(x-1)dy
$$
$$
=(\frac{1}{2}y^2-y)dx+(x-1)dy
$$
$$
=(\frac{1}{6}y^3-\frac{1}{2}y^2+x^2-x)dx+(x-1)dy
$$
$$
=(\frac{1}{6}y^3-\frac{1}{2}y^2+x^2-x)dx+(x-1)dy
$$
$$
=\frac{1}{6}y^3-\frac{1}{2}y^2+x^2-x-x+1
$$
$$
=\frac{1}{6}y^3-\frac{1}{2}y^2+x^2-2x+1
$$
$$
=\frac{1}{6}\times1^3-\frac{1}{2}\times1^2+1^2-2\times1+1
$$
$$
=\frac{1}{6}-\frac{1}{2}+1-2+1
$$
$$
=-\frac{1}{3}
$$